Resin.lean
@@ -1,1 +1,5 @@
-import Resin.Index
+import Resin.AddressMath
+import Resin.Front
+import Resin.ListVector
+import Resin.PNat
+import Resin.TensorLiteral
