Resin/Front.lean
@@ -1,0 +1,26 @@
+import Resin.AddressMath
+import Resin.TensorLiteral
+
+inductive Node : {rank : Nat} → Shape rank → Type where
+  | const
+      {rank : Nat}
+      {shape : Shape rank}
+      (literal : TensorLiteral shape)
+      : Node shape
+  | param
+      {rank : Nat}
+      {shape : Shape rank}
+      (id : Nat)
+      : Node shape
+  | view
+      {rank : Nat}
+      {shape : Shape rank}
+      {rank' : Nat}
+      {shape' : Shape rank'}
+      (src : Node shape')
+      : Node shape
+  | mul
+      {rank : Nat}
+      {shape : Shape rank}
+      (lhs rhs : Node shape)
+      : Node shape
