LEARN.md
@@ -1,0 +1,28 @@
+- [ ] How to use proof tactics? `by rfl`, `by simpa using ...`, etc.
+- [ ] How to explain this thing:
+
+  ```lean
+  inductive Node : {rank : Nat} → Shape rank → Type where
+    | const
+        {rank : Nat}
+        {shape : Shape rank}
+        (literal : TensorLiteral shape)
+        : Node shape
+    | param
+        {rank : Nat}
+        {shape : Shape rank}
+        (id : Nat)
+        : Node shape
+    | view
+        {rank : Nat}
+        {shape : Shape rank}
+        {rank' : Nat}
+        {shape' : Shape rank'}
+        (src : Node shape')
+        : Node shape
+    | mul
+        {rank : Nat}
+        {shape : Shape rank}
+        (lhs rhs : Node shape)
+        : Node shape
+  ```
